src/lang/Thread.v
@@ -62,7 +62,7 @@ Module Thread.
     Variable (lang:language).
 
     Structure t := mk {
-      state: lang.(Language.state);
+      state: (Language.state lang);
       local: Local.t;
       sc: TimeMap.t;
       memory: Memory.t;
@@ -84,7 +84,7 @@ Module Thread.
     | program_step_intro
         st1 lc1 sc1 mem1
         st2 lc2 sc2 mem2
-        (STATE: lang.(Language.step) (ThreadEvent.get_program_event e) st1 st2)
+        (STATE: (Language.step lang) (ThreadEvent.get_program_event e) st1 st2)
         (LOCAL: Local.program_step e lc1 sc1 mem1 lc2 sc2 mem2):
         program_step e (mk st1 lc1 sc1 mem1) (mk st2 lc2 sc2 mem2)
     .
@@ -191,12 +191,12 @@ Module Thread.
 
     Definition consistent (e:t): Prop :=
       forall mem1 sc1
-        (CAP: Memory.cap e.(local).(Local.promises) e.(memory) mem1)
+        (CAP: Memory.cap (Local.promises (local e)) (memory e) mem1)
         (SC_MAX: Memory.max_full_timemap mem1 sc1),
-        <<FAILURE: steps_failure (mk e.(state) e.(local) sc1 mem1)>> \/
+        <<FAILURE: steps_failure (mk (state e) (local e) sc1 mem1)>> \/
         exists e2,
-          <<STEPS: rtc tau_step (mk e.(state) e.(local) sc1 mem1) e2>> /\
-          <<PROMISES: e2.(local).(Local.promises) = Memory.bot>>.
+          <<STEPS: rtc tau_step (mk (state e) (local e) sc1 mem1) e2>> /\
+          <<PROMISES: (Local.promises (local e2)) = Memory.bot>>.
 
 
     (* step_future *)
@@ -204,15 +204,15 @@ Module Thread.
     Lemma promise_step_future
           pf e e1 e2
           (STEP: promise_step pf e e1 e2)
-          (WF1: Local.wf e1.(local) e1.(memory))
-          (SC1: Memory.closed_timemap e1.(sc) e1.(memory))
-          (CLOSED1: Memory.closed e1.(memory)):
-      <<WF2: Local.wf e2.(local) e2.(memory)>> /\
-      <<SC2: Memory.closed_timemap e2.(sc) e2.(memory)>> /\
-      <<CLOSED2: Memory.closed e2.(memory)>> /\
-      <<TVIEW_FUTURE: TView.le e1.(Thread.local).(Local.tview) e2.(Thread.local).(Local.tview)>> /\
-      <<SC_FUTURE: TimeMap.le e1.(sc) e2.(sc)>> /\
-      <<MEM_FUTURE: Memory.future e1.(memory) e2.(memory)>>.
+          (WF1: Local.wf (local e1) (memory e1))
+          (SC1: Memory.closed_timemap (sc e1) (memory e1))
+          (CLOSED1: Memory.closed (memory e1)):
+      <<WF2: Local.wf (local e2) (memory e2)>> /\
+      <<SC2: Memory.closed_timemap (sc e2) (memory e2)>> /\
+      <<CLOSED2: Memory.closed (memory e2)>> /\
+      <<TVIEW_FUTURE: TView.le (Local.tview (Thread.local e1)) (Local.tview (Thread.local e2))>> /\
+      <<SC_FUTURE: TimeMap.le (sc e1) (sc e2)>> /\
+      <<MEM_FUTURE: Memory.future (memory e1) (memory e2)>>.
     Proof.
       inv STEP. ss.
       exploit Local.promise_step_future; eauto. i. des.
@@ -222,15 +222,15 @@ Module Thread.
     Lemma program_step_future
           e e1 e2
           (STEP: program_step e e1 e2)
-          (WF1: Local.wf e1.(local) e1.(memory))
-          (SC1: Memory.closed_timemap e1.(sc) e1.(memory))
-          (CLOSED1: Memory.closed e1.(memory)):
-      <<WF2: Local.wf e2.(local) e2.(memory)>> /\
-      <<SC2: Memory.closed_timemap e2.(sc) e2.(memory)>> /\
-      <<CLOSED2: Memory.closed e2.(memory)>> /\
-      <<TVIEW_FUTURE: TView.le e1.(Thread.local).(Local.tview) e2.(Thread.local).(Local.tview)>> /\
-      <<SC_FUTURE: TimeMap.le e1.(sc) e2.(sc)>> /\
-      <<MEM_FUTURE: Memory.future e1.(memory) e2.(memory)>>.
+          (WF1: Local.wf (local e1) (memory e1))
+          (SC1: Memory.closed_timemap (sc e1) (memory e1))
+          (CLOSED1: Memory.closed (memory e1)):
+      <<WF2: Local.wf (local e2) (memory e2)>> /\
+      <<SC2: Memory.closed_timemap (sc e2) (memory e2)>> /\
+      <<CLOSED2: Memory.closed (memory e2)>> /\
+      <<TVIEW_FUTURE: TView.le (Local.tview (Thread.local e1)) (Local.tview (Thread.local e2))>> /\
+      <<SC_FUTURE: TimeMap.le (sc e1) (sc e2)>> /\
+      <<MEM_FUTURE: Memory.future (memory e1) (memory e2)>>.
     Proof.
       inv STEP. ss. eapply Local.program_step_future; eauto.
     Qed.
@@ -238,15 +238,15 @@ Module Thread.
     Lemma step_future
           pf e e1 e2
           (STEP: step pf e e1 e2)
-          (WF1: Local.wf e1.(local) e1.(memory))
-          (SC1: Memory.closed_timemap e1.(sc) e1.(memory))
-          (CLOSED1: Memory.closed e1.(memory)):
-      <<WF2: Local.wf e2.(local) e2.(memory)>> /\
-      <<SC2: Memory.closed_timemap e2.(sc) e2.(memory)>> /\
-      <<CLOSED2: Memory.closed e2.(memory)>> /\
-      <<TVIEW_FUTURE: TView.le e1.(Thread.local).(Local.tview) e2.(Thread.local).(Local.tview)>> /\
-      <<SC_FUTURE: TimeMap.le e1.(sc) e2.(sc)>> /\
-      <<MEM_FUTURE: Memory.future e1.(memory) e2.(memory)>>.
+          (WF1: Local.wf (local e1) (memory e1))
+          (SC1: Memory.closed_timemap (sc e1) (memory e1))
+          (CLOSED1: Memory.closed (memory e1)):
+      <<WF2: Local.wf (local e2) (memory e2)>> /\
+      <<SC2: Memory.closed_timemap (sc e2) (memory e2)>> /\
+      <<CLOSED2: Memory.closed (memory e2)>> /\
+      <<TVIEW_FUTURE: TView.le (Local.tview (Thread.local e1)) (Local.tview (Thread.local e2))>> /\
+      <<SC_FUTURE: TimeMap.le (sc e1) (sc e2)>> /\
+      <<MEM_FUTURE: Memory.future (memory e1) (memory e2)>>.
     Proof.
       inv STEP.
       - eapply promise_step_future; eauto.
@@ -256,15 +256,15 @@ Module Thread.
     Lemma opt_step_future
           e e1 e2
           (STEP: opt_step e e1 e2)
-          (WF1: Local.wf e1.(local) e1.(memory))
-          (SC1: Memory.closed_timemap e1.(sc) e1.(memory))
-          (CLOSED1: Memory.closed e1.(memory)):
-      <<WF2: Local.wf e2.(local) e2.(memory)>> /\
-      <<SC2: Memory.closed_timemap e2.(sc) e2.(memory)>> /\
-      <<CLOSED2: Memory.closed e2.(memory)>> /\
-      <<TVIEW_FUTURE: TView.le e1.(Thread.local).(Local.tview) e2.(Thread.local).(Local.tview)>> /\
-      <<SC_FUTURE: TimeMap.le e1.(sc) e2.(sc)>> /\
-      <<MEM_FUTURE: Memory.future e1.(memory) e2.(memory)>>.
+          (WF1: Local.wf (local e1) (memory e1))
+          (SC1: Memory.closed_timemap (sc e1) (memory e1))
+          (CLOSED1: Memory.closed (memory e1)):
+      <<WF2: Local.wf (local e2) (memory e2)>> /\
+      <<SC2: Memory.closed_timemap (sc e2) (memory e2)>> /\
+      <<CLOSED2: Memory.closed (memory e2)>> /\
+      <<TVIEW_FUTURE: TView.le (Local.tview (Thread.local e1)) (Local.tview (Thread.local e2))>> /\
+      <<SC_FUTURE: TimeMap.le (sc e1) (sc e2)>> /\
+      <<MEM_FUTURE: Memory.future (memory e1) (memory e2)>>.
     Proof.
       inv STEP.
       - esplits; eauto; refl.
@@ -274,15 +274,15 @@ Module Thread.
     Lemma rtc_all_step_future
           e1 e2
           (STEP: rtc all_step e1 e2)
-          (WF1: Local.wf e1.(local) e1.(memory))
-          (SC1: Memory.closed_timemap e1.(sc) e1.(memory))
-          (CLOSED1: Memory.closed e1.(memory)):
-      <<WF2: Local.wf e2.(local) e2.(memory)>> /\
-      <<SC2: Memory.closed_timemap e2.(sc) e2.(memory)>> /\
-      <<CLOSED2: Memory.closed e2.(memory)>> /\
-      <<TVIEW_FUTURE: TView.le e1.(Thread.local).(Local.tview) e2.(Thread.local).(Local.tview)>> /\
-      <<SC_FUTURE: TimeMap.le e1.(sc) e2.(sc)>> /\
-      <<MEM_FUTURE: Memory.future e1.(memory) e2.(memory)>>.
+          (WF1: Local.wf (local e1) (memory e1))
+          (SC1: Memory.closed_timemap (sc e1) (memory e1))
+          (CLOSED1: Memory.closed (memory e1)):
+      <<WF2: Local.wf (local e2) (memory e2)>> /\
+      <<SC2: Memory.closed_timemap (sc e2) (memory e2)>> /\
+      <<CLOSED2: Memory.closed (memory e2)>> /\
+      <<TVIEW_FUTURE: TView.le (Local.tview (Thread.local e1)) (Local.tview (Thread.local e2))>> /\
+      <<SC_FUTURE: TimeMap.le (sc e1) (sc e2)>> /\
+      <<MEM_FUTURE: Memory.future (memory e1) (memory e2)>>.
     Proof.
       revert WF1. induction STEP.
       - i. splits; ss; refl.
@@ -295,15 +295,15 @@ Module Thread.
     Lemma rtc_tau_step_future
           e1 e2
           (STEP: rtc tau_step e1 e2)
-          (WF1: Local.wf e1.(local) e1.(memory))
-          (SC1: Memory.closed_timemap e1.(sc) e1.(memory))
-          (CLOSED1: Memory.closed e1.(memory)):
-      <<WF2: Local.wf e2.(local) e2.(memory)>> /\
-      <<SC2: Memory.closed_timemap e2.(sc) e2.(memory)>> /\
-      <<CLOSED2: Memory.closed e2.(memory)>> /\
-      <<TVIEW_FUTURE: TView.le e1.(Thread.local).(Local.tview) e2.(Thread.local).(Local.tview)>> /\
-      <<SC_FUTURE: TimeMap.le e1.(sc) e2.(sc)>> /\
-      <<MEM_FUTURE: Memory.future e1.(memory) e2.(memory)>>.
+          (WF1: Local.wf (local e1) (memory e1))
+          (SC1: Memory.closed_timemap (sc e1) (memory e1))
+          (CLOSED1: Memory.closed (memory e1)):
+      <<WF2: Local.wf (local e2) (memory e2)>> /\
+      <<SC2: Memory.closed_timemap (sc e2) (memory e2)>> /\
+      <<CLOSED2: Memory.closed (memory e2)>> /\
+      <<TVIEW_FUTURE: TView.le (Local.tview (Thread.local e1)) (Local.tview (Thread.local e2))>> /\
+      <<SC_FUTURE: TimeMap.le (sc e1) (sc e2)>> /\
+      <<MEM_FUTURE: Memory.future (memory e1) (memory e2)>>.
     Proof.
       apply rtc_all_step_future; auto.
       eapply rtc_implies; [|eauto].
@@ -316,8 +316,8 @@ Module Thread.
     Lemma promise_step_inhabited
           pf e e1 e2
           (STEP: promise_step pf e e1 e2)
-          (INHABITED1: Memory.inhabited e1.(memory)):
-      <<INHABITED2: Memory.inhabited e2.(memory)>>.
+          (INHABITED1: Memory.inhabited (memory e1)):
+      <<INHABITED2: Memory.inhabited (memory e2)>>.
     Proof.
       inv STEP. ss.
       eapply Local.promise_step_inhabited; eauto.
@@ -326,8 +326,8 @@ Module Thread.
     Lemma program_step_inhabited
           e e1 e2
           (STEP: program_step e e1 e2)
-          (INHABITED1: Memory.inhabited e1.(memory)):
-      <<INHABITED2: Memory.inhabited e2.(memory)>>.
+          (INHABITED1: Memory.inhabited (memory e1)):
+      <<INHABITED2: Memory.inhabited (memory e2)>>.
     Proof.
       inv STEP. ss.
       eapply Local.program_step_inhabited; eauto.
@@ -336,8 +336,8 @@ Module Thread.
     Lemma step_inhabited
           pf e e1 e2
           (STEP: step pf e e1 e2)
-          (INHABITED1: Memory.inhabited e1.(memory)):
-      <<INHABITED2: Memory.inhabited e2.(memory)>>.
+          (INHABITED1: Memory.inhabited (memory e1)):
+      <<INHABITED2: Memory.inhabited (memory e2)>>.
     Proof.
       inv STEP.
       - eapply promise_step_inhabited; eauto.
@@ -350,13 +350,13 @@ Module Thread.
     Lemma promise_step_disjoint
           pf e e1 e2 lc
           (STEP: promise_step pf e e1 e2)
-          (WF1: Local.wf e1.(local) e1.(memory))
-          (SC1: Memory.closed_timemap e1.(sc) e1.(memory))
-          (CLOSED1: Memory.closed e1.(memory))
-          (DISJOINT1: Local.disjoint e1.(local) lc)
-          (WF: Local.wf lc e1.(memory)):
-      <<DISJOINT2: Local.disjoint e2.(local) lc>> /\
-      <<WF: Local.wf lc e2.(memory)>>.
+          (WF1: Local.wf (local e1) (memory e1))
+          (SC1: Memory.closed_timemap (sc e1) (memory e1))
+          (CLOSED1: Memory.closed (memory e1))
+          (DISJOINT1: Local.disjoint (local e1) lc)
+          (WF: Local.wf lc (memory e1)):
+      <<DISJOINT2: Local.disjoint (local e2) lc>> /\
+      <<WF: Local.wf lc (memory e2)>>.
     Proof.
       inv STEP.
       exploit Local.promise_step_future; eauto. i. des.
@@ -366,13 +366,13 @@ Module Thread.
     Lemma program_step_disjoint
           e e1 e2 lc
           (STEP: program_step e e1 e2)
-          (WF1: Local.wf e1.(local) e1.(memory))
-          (SC1: Memory.closed_timemap e1.(sc) e1.(memory))
-          (CLOSED1: Memory.closed e1.(memory))
-          (DISJOINT1: Local.disjoint e1.(local) lc)
-          (WF: Local.wf lc e1.(memory)):
-      <<DISJOINT2: Local.disjoint e2.(local) lc>> /\
-      <<WF: Local.wf lc e2.(memory)>>.
+          (WF1: Local.wf (local e1) (memory e1))
+          (SC1: Memory.closed_timemap (sc e1) (memory e1))
+          (CLOSED1: Memory.closed (memory e1))
+          (DISJOINT1: Local.disjoint (local e1) lc)
+          (WF: Local.wf lc (memory e1)):
+      <<DISJOINT2: Local.disjoint (local e2) lc>> /\
+      <<WF: Local.wf lc (memory e2)>>.
     Proof.
       inv STEP. ss. eapply Local.program_step_disjoint; eauto.
     Qed.
@@ -380,13 +380,13 @@ Module Thread.
     Lemma step_disjoint
           pf e e1 e2 lc
           (STEP: step pf e e1 e2)
-          (WF1: Local.wf e1.(local) e1.(memory))
-          (SC1: Memory.closed_timemap e1.(sc) e1.(memory))
-          (CLOSED1: Memory.closed e1.(memory))
-          (DISJOINT1: Local.disjoint e1.(local) lc)
-          (WF: Local.wf lc e1.(memory)):
-      <<DISJOINT2: Local.disjoint e2.(local) lc>> /\
-      <<WF: Local.wf lc e2.(memory)>>.
+          (WF1: Local.wf (local e1) (memory e1))
+          (SC1: Memory.closed_timemap (sc e1) (memory e1))
+          (CLOSED1: Memory.closed (memory e1))
+          (DISJOINT1: Local.disjoint (local e1) lc)
+          (WF: Local.wf lc (memory e1)):
+      <<DISJOINT2: Local.disjoint (local e2) lc>> /\
+      <<WF: Local.wf lc (memory e2)>>.
     Proof.
       inv STEP.
       - eapply promise_step_disjoint; eauto.
@@ -396,13 +396,13 @@ Module Thread.
     Lemma opt_step_disjoint
           e e1 e2 lc
           (STEP: opt_step e e1 e2)
-          (WF1: Local.wf e1.(local) e1.(memory))
-          (SC1: Memory.closed_timemap e1.(sc) e1.(memory))
-          (CLOSED1: Memory.closed e1.(memory))
-          (DISJOINT1: Local.disjoint e1.(local) lc)
-          (WF: Local.wf lc e1.(memory)):
-      <<DISJOINT2: Local.disjoint e2.(local) lc>> /\
-      <<WF: Local.wf lc e2.(memory)>>.
+          (WF1: Local.wf (local e1) (memory e1))
+          (SC1: Memory.closed_timemap (sc e1) (memory e1))
+          (CLOSED1: Memory.closed (memory e1))
+          (DISJOINT1: Local.disjoint (local e1) lc)
+          (WF: Local.wf lc (memory e1)):
+      <<DISJOINT2: Local.disjoint (local e2) lc>> /\
+      <<WF: Local.wf lc (memory e2)>>.
     Proof.
       inv STEP.
       - esplits; eauto.
@@ -412,13 +412,13 @@ Module Thread.
     Lemma rtc_all_step_disjoint
           e1 e2 lc
           (STEP: rtc all_step e1 e2)
-          (WF1: Local.wf e1.(local) e1.(memory))
-          (SC1: Memory.closed_timemap e1.(sc) e1.(memory))
-          (CLOSED1: Memory.closed e1.(memory))
-          (DISJOINT1: Local.disjoint e1.(local) lc)
-          (WF: Local.wf lc e1.(memory)):
-      <<DISJOINT2: Local.disjoint e2.(local) lc>> /\
-      <<WF: Local.wf lc e2.(memory)>>.
+          (WF1: Local.wf (local e1) (memory e1))
+          (SC1: Memory.closed_timemap (sc e1) (memory e1))
+          (CLOSED1: Memory.closed (memory e1))
+          (DISJOINT1: Local.disjoint (local e1) lc)
+          (WF: Local.wf lc (memory e1)):
+      <<DISJOINT2: Local.disjoint (local e2) lc>> /\
+      <<WF: Local.wf lc (memory e2)>>.
     Proof.
       revert WF1 DISJOINT1 WF. induction STEP; eauto. i.
       inv H. inv USTEP.
@@ -430,13 +430,13 @@ Module Thread.
     Lemma rtc_tau_step_disjoint
           e1 e2 lc
           (STEP: rtc tau_step e1 e2)
-          (WF1: Local.wf e1.(local) e1.(memory))
-          (SC1: Memory.closed_timemap e1.(sc) e1.(memory))
-          (CLOSED1: Memory.closed e1.(memory))
-          (DISJOINT1: Local.disjoint e1.(local) lc)
-          (WF: Local.wf lc e1.(memory)):
-      <<DISJOINT2: Local.disjoint e2.(local) lc>> /\
-      <<WF: Local.wf lc e2.(memory)>>.
+          (WF1: Local.wf (local e1) (memory e1))
+          (SC1: Memory.closed_timemap (sc e1) (memory e1))
+          (CLOSED1: Memory.closed (memory e1))
+          (DISJOINT1: Local.disjoint (local e1) lc)
+          (WF: Local.wf lc (memory e1)):
+      <<DISJOINT2: Local.disjoint (local e2) lc>> /\
+      <<WF: Local.wf lc (memory e2)>>.
     Proof.
       eapply rtc_all_step_disjoint; cycle 1; eauto.
       eapply rtc_implies; [|eauto].
@@ -447,12 +447,12 @@ Module Thread.
     (* step_no_reserve_except *)
 
     Definition no_reserve_except (e: t) :=
-      Memory.no_reserve_except e.(local).(Local.promises) e.(memory).
+      Memory.no_reserve_except (Local.promises (local e)) (memory e).
 
     Lemma step_no_reserve_except
           pf e e1 e2
           (STEP: step pf e e1 e2)
-          (WF1: Local.wf e1.(local) e1.(memory))
+          (WF1: Local.wf (local e1) (memory e1))
           (NORESERVE1: no_reserve_except e1):
       no_reserve_except e2.
     Proof.
@@ -464,9 +464,9 @@ Module Thread.
     Lemma rtc_tau_step_no_reserve_except
           e1 e2
           (STEP: rtc tau_step e1 e2)
-          (WF1: Local.wf e1.(local) e1.(memory))
-          (SC1: Memory.closed_timemap e1.(sc) e1.(memory))
-          (CLOSED1: Memory.closed e1.(memory))
+          (WF1: Local.wf (local e1) (memory e1))
+          (SC1: Memory.closed_timemap (sc e1) (memory e1))
+          (CLOSED1: Memory.closed (memory e1))
           (NORESERVE1: no_reserve_except e1):
       no_reserve_except e2.
     Proof.
@@ -479,12 +479,12 @@ Module Thread.
     Lemma step_bot_no_reserve
           pf e e1 e2
           (STEP: step pf e e1 e2)
-          (WF1: Local.wf e1.(local) e1.(memory))
-          (SC1: Memory.closed_timemap e1.(sc) e1.(memory))
-          (CLOSED1: Memory.closed e1.(memory))
-          (NORESERVE1: Memory.no_reserve e1.(memory))
-          (PROMISES2: e2.(local).(Local.promises) = Memory.bot):
-      Memory.no_reserve e2.(memory).
+          (WF1: Local.wf (local e1) (memory e1))
+          (SC1: Memory.closed_timemap (sc e1) (memory e1))
+          (CLOSED1: Memory.closed (memory e1))
+          (NORESERVE1: Memory.no_reserve (memory e1))
+          (PROMISES2: (Local.promises (local e2)) = Memory.bot):
+      Memory.no_reserve (memory e2).
     Proof.
       exploit step_future; eauto. i. des.
       hexploit step_no_reserve_except; eauto; i.
@@ -497,12 +497,12 @@ Module Thread.
     Lemma rtc_tau_step_bot_no_reserve
           e1 e2
           (STEP: rtc tau_step e1 e2)
-          (WF1: Local.wf e1.(local) e1.(memory))
-          (SC1: Memory.closed_timemap e1.(sc) e1.(memory))
-          (CLOSED1: Memory.closed e1.(memory))
-          (NORESERVE1: Memory.no_reserve e1.(memory))
-          (PROMISES2: e2.(local).(Local.promises) = Memory.bot):
-      Memory.no_reserve e2.(memory).
+          (WF1: Local.wf (local e1) (memory e1))
+          (SC1: Memory.closed_timemap (sc e1) (memory e1))
+          (CLOSED1: Memory.closed (memory e1))
+          (NORESERVE1: Memory.no_reserve (memory e1))
+          (PROMISES2: (Local.promises (local e2)) = Memory.bot):
+      Memory.no_reserve (memory e2).
     Proof.
       exploit rtc_tau_step_future; eauto. i. des.
       hexploit rtc_tau_step_no_reserve_except; eauto; i.
@@ -515,8 +515,8 @@ Module Thread.
     Lemma program_step_promises_bot
           e e1 e2
           (STEP: program_step e e1 e2)
-          (PROMISES: e1.(local).(Local.promises) = Memory.bot):
-      e2.(local).(Local.promises) = Memory.bot.
+          (PROMISES: (Local.promises (local e1)) = Memory.bot):
+      (Local.promises (local e2)) = Memory.bot.
     Proof.
       inv STEP. eapply Local.program_step_promises_bot; eauto.
     Qed.
@@ -527,7 +527,7 @@ Module Thread.
     Lemma step_prev_None
           pf e e1 e2
           (STEP: step pf e e1 e2):
-      <<PREV: Memory.prev_None e1.(memory) e2.(memory)>>.
+      <<PREV: Memory.prev_None (memory e1) (memory e2)>>.
     Proof.
       inv STEP; inv STEP0; inv LOCAL; ss;
         try by ii; eapply GET_PREV; eauto.
@@ -541,7 +541,7 @@ Module Thread.
     Lemma opt_step_prev_None
           e e1 e2
           (STEP: opt_step e e1 e2):
-      <<PREV: Memory.prev_None e1.(memory) e2.(memory)>>.
+      <<PREV: Memory.prev_None (memory e1) (memory e2)>>.
     Proof.
       inv STEP; eauto using step_prev_None.
       ii. eapply GET_PREV; eauto.
@@ -550,7 +550,7 @@ Module Thread.
     Lemma rtc_tau_step_prev_None
           e1 e2
           (STEPS: rtc tau_step e1 e2):
-      <<PREV: Memory.prev_None e1.(memory) e2.(memory)>>.
+      <<PREV: Memory.prev_None (memory e1) (memory e2)>>.
     Proof.
       induction STEPS.
       - ii. eapply GET_PREV; eauto.
@@ -572,7 +572,7 @@ Module Thread.
     Lemma rtc_all_step_prev_None
           e1 e2
           (STEPS: rtc all_step e1 e2):
-      <<PREV: Memory.prev_None e1.(memory) e2.(memory)>>.
+      <<PREV: Memory.prev_None (memory e1) (memory e2)>>.
     Proof.
       induction STEPS.
       - ii. eapply GET_PREV; eauto.
