src/pf/APF.v
@@ -30,10 +30,10 @@ Module APFConfiguration.
   Inductive step: forall (e:MachineEvent.t) (tid:Ident.t) (c1 c2: Configuration.t), Prop :=
   | step_intro
       e tid c1 lang st1 lc1 e2 st3 lc3 sc3 memory3
-      (TID: IdentMap.find tid c1.(Configuration.threads) = Some (existT _ lang st1, lc1))
-      (STEPS: rtc (tau (@AThread.program_step _)) (Thread.mk _ st1 lc1 c1.(Configuration.sc) c1.(Configuration.memory)) e2)
+      (TID: IdentMap.find tid (Configuration.threads c1) = Some (existT _ lang st1, lc1))
+      (STEPS: rtc (tau (@AThread.program_step _)) (Thread.mk _ st1 lc1 (Configuration.sc c1) (Configuration.memory c1)) e2)
       (STEP: AThread.program_step e e2 (Thread.mk _ st3 lc3 sc3 memory3)):
-      step (ThreadEvent.get_machine_event e) tid c1 (Configuration.mk (IdentMap.add tid (existT _ _ st3, lc3) c1.(Configuration.threads)) sc3 memory3)
+      step (ThreadEvent.get_machine_event e) tid c1 (Configuration.mk (IdentMap.add tid (existT _ _ st3, lc3) (Configuration.threads c1)) sc3 memory3)
   .
   Hint Constructors step.
 
@@ -107,9 +107,9 @@ Module APFConfiguration.
 
   Lemma program_step_no_promise lang (th0 th1: Thread.t lang) e
         (STEP: AThread.program_step e th0 th1)
-        (NOPROMISE: th0.(Thread.local).(Local.promises) = Memory.bot)
+        (NOPROMISE: (Local.promises (Thread.local th0)) = Memory.bot)
     :
-      th1.(Thread.local).(Local.promises) = Memory.bot.
+      (Local.promises (Thread.local th1)) = Memory.bot.
   Proof.
     inv STEP. inv LOCAL; ss.
     - inv LOCAL0. ss.
@@ -123,9 +123,9 @@ Module APFConfiguration.
 
   Lemma program_steps_no_promise lang (th0 th1: Thread.t lang)
         (STEP: rtc (tau (@AThread.program_step lang)) th0 th1)
-        (NOPROMISE: th0.(Thread.local).(Local.promises) = Memory.bot)
+        (NOPROMISE: (Local.promises (Thread.local th0)) = Memory.bot)
     :
-      th1.(Thread.local).(Local.promises) = Memory.bot.
+      (Local.promises (Thread.local th1)) = Memory.bot.
   Proof.
     ginduction STEP; ss. i. eapply IHSTEP. inv H.
     eapply program_step_no_promise; eauto.
@@ -136,7 +136,7 @@ Module APFConfiguration.
         tid st lc
         (FIND: IdentMap.find tid (Configuration.threads c) = Some (st, lc))
     :
-      lc.(Local.promises) = Memory.bot.
+      (Local.promises lc) = Memory.bot.
   Proof.
     eapply Memory.ext. i. rewrite Memory.bot_get.
     destruct (Memory.get loc ts (Local.promises lc)) as [[from msg]|] eqn:GET; auto.
