src/opt/SimPromises.v
@@ -538,14 +538,14 @@ Module SimPromises.
         pview
         lc_src mem1_src mem2_src
         lc_tgt mem1_tgt
-        (INV1: sem pview bot lc_src.(Local.promises) lc_tgt.(Local.promises))
+        (INV1: sem pview bot (Local.promises lc_src) (Local.promises lc_tgt))
         (MEM1: sim_memory mem1_src mem1_tgt)
-        (CAP_SRC: Memory.cap lc_src.(Local.promises) mem1_src mem2_src)
+        (CAP_SRC: Memory.cap (Local.promises lc_src) mem1_src mem2_src)
         (MEM1_SRC: Memory.closed mem1_src)
         (MEM1_TGT: Memory.closed mem1_tgt):
     exists mem2_tgt,
       <<MEM2: sim_memory mem2_src mem2_tgt>> /\
-      <<CAP_TGT: Memory.cap lc_tgt.(Local.promises) mem1_tgt mem2_tgt>>.
+      <<CAP_TGT: Memory.cap (Local.promises lc_tgt) mem1_tgt mem2_tgt>>.
   Proof.
     exploit Memory.cap_exists; try exact MEM1_TGT; eauto. i. des.
     esplits; eauto.
